code/Transitions.v
@@ -1,0 +1,70 @@
+
+(*************************************************************************)
+(** * Transition Systems (PFPL 5.1) *)
+(*************************************************************************)
+
+(* The beginning of Ch5 introduces general terminology for reasoning about 
+   the evaluation of programs.  We can capture the generality of these 
+   definition using Coq's module system. The following module type 
+   defines what it means to be a transition system in abstract terms. 
+ *)
+
+Module Type TransitionSystem.
+  Parameter S : Set.
+  Parameter state : S -> Prop.
+
+  Parameter final : S -> Prop.
+  Axiom final_state : forall s, final s -> state s.
+
+  Parameter initial : S -> Prop.
+  Axiom initial_state : forall s, initial s -> state s.
+  
+  Parameter step : S -> S -> Prop.
+  Axiom step_states : forall s1 s2, step s1 s2 -> state s1 /\ state s2.
+
+  Axiom final_does_not_step : forall s, final s -> not (exists s', step s s').    
+  
+End TransitionSystem.
+
+(* Once we know what a transition system is, we can define terminolody
+   and prove theorems in terms of the basic definitions above. *)
+
+Module TransitionSystemProperties (TS : TransitionSystem).
+  Import TS.
+
+  Definition stuck (s : S) :=
+    not (final s) /\ not (exists s', step s s').
+
+  (* The multistep relation describes a sequence of transitions. *)
+  Inductive multistep : S -> S -> Prop :=
+    | ms_refl : forall s, state s -> multistep s s
+    | ms_step : forall s s' s'', step s s' -> multistep s' s'' -> multistep s s''.        
+  Hint Constructors multistep.
+  
+  Lemma multistep_transitive : forall s s' s'',
+      multistep s s' -> multistep s' s'' -> multistep s s''.
+  Proof.
+    intros s s' s'' MS1 MS2.
+    induction MS1; eauto.
+  Qed.
+
+  Lemma multistep_states : forall s1 s2, multistep s1 s2 -> state s1 /\ state s2.
+  Proof.
+    intros s1 s2 MS. induction MS. auto. split.
+    destruct (step_states _ _ H). auto. destruct IHMS. auto.
+  Qed.
+
+  (* We say with this is a transition sequence if the first state 
+     is initial. *)
+  Definition transition_sequence s s' (ms : multistep s s') := initial s.
+
+  (* It is a maximial transition sequence if the last state doesn't step. *)
+  Definition maximal_transition_sequence s s' (ms : multistep s s') :=
+    initial s /\ not (exists s'', step s' s'').
+
+  (* And a complete transition sequence if the last step is final *)
+  Definition complete_transition_sequence s s' (ms : multistep s s') :=
+    initial s /\ final s'.
+  
+
+End TransitionSystemProperties.  
